---
layout: subpage
title: Proposition:<br/> For \(s_{n + 1}\) \( = s_n \) \( + \dfrac{1}{2}(x - {s_n}^2)\), prove that \(s_n\) converges
description: Discusses the given proposition, the intuition behind the proof, and the proof itself
---

In this section, I will discuss the given proposition, the intuition behind the proof, and the
proof itself.

---

_**Proposition**_

Let $$x$$ be a real number so that $$0 \leqslant x$$ $$ \leqslant 1$$. Define a
sequence $$(s_n)_{n=1}^\infty$$ by $$s_1 = 0$$,
$$s_{n + 1} = s_n + \dfrac{1}{2}(x - {s_n}^2)$$ for $$n \in \mathbb{N}$$.

Show that $$(s_n)_{n=1}^\infty$$ is a monotone bounded sequence and hence converges
to some $$s \in \mathbb{R}$$. Show that $$s^2 = x$$.

[//]: # _**Intuition**_

_**Proof**_

First, we show that $$s_n$$ is bounded above.

(Claim: $$s_n \leqslant 1$$ $$(\forall n \in \mathbb{N})$$

Base Case:

$$s_1 = 0$$ $$ \leqslant 1$$, is obviously true.

Inductive Case:

Assume inductively, that, $$s_k \leqslant 1$$.

Then, $$s_{k + 1} = s_k + \dfrac{1}{2}(x- {s_k}^2)$$
$$ = s_k + \dfrac{1}{2}x - \dfrac{1}{2}{s_k}^2$$
$$ = s_k - \dfrac{1}{2}{s_k}^2 + \dfrac{1}{2}x$$
$$ = -\left(\dfrac{1}{2}{s_k}^2 - s_k\right) + \dfrac{1}{2}x$$
$$ = -\left(\dfrac{1}{2}(s_k - 1)^2\right) + \dfrac{1}{2} + \dfrac{1}{2}x$$
$$ = \dfrac{1}{2} - \dfrac{1}{2}(s_k - 1)^2 + \dfrac{1}{2}x$$
$$ \leqslant \dfrac{1}{2} + \dfrac{1}{2}x$$ $$ \leqslant 1$$ (since, $$x \leqslant 1$$).

Hence, this shows that $$s_n \leqslant 1$$ $$(\forall n \in \mathbb{N})$$, is
bounded above (by 1).

Next, we show monotonicity, specifically, that $$(s_n)_{n=1}^\infty$$ is nondecreasing.

(Claim: $$s_n \leqslant s_{n + 1}$$)

Base Case:

$$s_1 = 0$$ $$ \leqslant s_1 = 0 + \dfrac{1}{2}(x - 0^2)$$
$$ = \dfrac{1}{2}x$$ (where $$0 \leqslant x$$ $$ \leqslant 1$$).

Inductive Case:

Inductively, assume that, $$s_k \leqslant s_{k + 1}$$, then, we note that,

$$s_{k + 1} = s_k + \dfrac{1}{2}(x - {s_k}^2)$$ $$\ldots (1)$$

$$s_{k + 2} = s_{k + 1} + \dfrac{1}{2}(x - {s_{k + 1}}^2)$$ $$\ldots (2)$$.

$$(2) - (1) = s_{k + 2} - s_{k + 1}$$
$$ = s_{k + 1} + \dfrac{1}{2}(x - {s_{k + 1}}^2) - \left(s_k + \dfrac{1}{2}(x - {s_k}^2)\right)$$
$$ = s_{k + 1} + \dfrac{1}{2}(x - {s_{k + 1}}^2) - s_k - \dfrac{1}{2}(x - {s_k}^2)$$
$$ = s_{k + 1} + \dfrac{1}{2}x - \dfrac{1}{2}{s_{k + 1}}^2 - s_k - \dfrac{1}{2}x + \dfrac{1}{2}{s_k}^2$$
$$ = (s_{k + 1} - s_k) - \dfrac{1}{2}({s_{k + 1}}^2 - {s_k}^2)$$
$$ = (s_{k + 1} - s_k) - \dfrac{1}{2}[(s_{k + 1} + s_k)(s_{k + 1} - s_k)]$$
$$ = (s_{k + 1} - s_k)\left(1 - \dfrac{1}{2}(s_{k + 1} + s_k)\right)$$ $$ ...(3)$$

But, since, we know that $$s_n \leqslant 1$$ $$(\forall n \in \mathbb{N})$$,
$$s_k + s_{k + 1} \leqslant 2$$ $$\Longrightarrow \dfrac{1}{2}(s_k + s_{k + 1}) \leqslant 1$$
$$ => 1 - \dfrac{1}{2}(s_k + s_{k + 1}) \geqslant 0$$.

Also, $$s_{k + 1} - s_k \geqslant 0$$, from our inductive hypothesis; $$s_k \leqslant s_{k + 1}$$.

Thus, $$s_{k + 2} - s_{k + 1} = (3)$$ $$ \geqslant 0$$ $$ => s_{k + 2} - s_{k + 1} \geqslant 0$$
$$ => s_{k + 2} \geqslant s_{k + 1}$$ $$ => s_{k + 1} \leqslant s_{k + 2}$$.

Hence, this proves that $$(s_n)_{n=1}^\infty$$ is nondecreasing.

Thus, since $$(s_n)_{n=1}^\infty$$ is nondecreasing and bounded above, it is convergent to some
$$s \in \mathbb{R}$$.

Now, take limits on both sides of this equation;
$$s_{n + 1} = s_n + \dfrac{1}{2}(x - {s_n}^2)$$, and we obtain,
$$\lim\limits_{n \to \infty} s_{n + 1} = \lim\limits_{n \to \infty}\left(s_n + \dfrac{1}{2}(x - {s_n}^2)\right)$$
$$\Longrightarrow \lim\limits_{n \to \infty} s_{n + 1} = \lim\limits_{n \to \infty} s_n + \dfrac{1}{2}\lim\limits_{n \to \infty} x - \dfrac{1}{2}\lim\limits_{n \to \infty} {s_n}^2$$
$$\Longrightarrow s = s + \dfrac{1}{2}x - \dfrac{1}{2}s^2$$
(since,  $$(s_{n + 1})_{n=1}^\infty$$ is a subsequence of $$(s_n)_{n=1}^\infty$$)
$$\Longrightarrow \dfrac{1}{2}s^2 = \dfrac{1}{2}x$$ $$\Longrightarrow s^2 = x$$, as needed. $$\blacksquare$$
