---
layout: subpage
title: Richard Goldberg Exercise 2.7 Q10(c)
description: Discusses the given question, the intuition behind the proof, and the proof itself
---

In this section, I will discuss the given question, the intuition behind the proof, and the
proof itself.

---

**Question**

Suppose $$s_1 > s_2$$ $$> 0$$, and let $$s_{n + 1} = \dfrac{1}{2} (s_n + s_{n - 1})$$
$$(n \geqslant 2)$$.

Prove that $$(s_n)_{n=1}^\infty$$ is convergent.

**Proof**

We note that the terms in the sequence are bounded by the closed interval;
$$[s_2, s_1]$$.

This implies that the even and odd subsequences are bounded as well.

But since they are monotonic, they are convergent to some,
$$L, M \in \mathbb{R}$$ respectively.

But, $$\lim\limits_{n \to \infty} s_{2n - 1} = \lim\limits_{n \to \infty} s_{2n}$$,
since $$(s_{2n})_{n=1}^\infty$$ is a subsequence of $$(s_{2n - 1})_{n=1}^\infty$$,
by the formulae of the original sequence.

Hence, $$L = M$$, and the original sequence $$(s_n)_{n=1}^\infty$$ converges
(to $$L \in \mathbb{R}$$).
