---
layout: subpage
title: Richard Goldberg Exercise 2.6 Q6
description: Discusses the given question, the intuition behind the proof, and the proof itself
---

In this section, I will discuss the given question, the intuition behind the proof, and the
proof itself.

---

_**Question**_

For $$n \in \mathbb{N}$$,
let $$s_n = \dfrac{1 \cdot 3 \cdot 5 \cdot \cdot \cdot (2n - 1)}{2 \cdot 4 \cdot 6 \cdot \cdot \cdot 2n}$$.

Prove that
$$(s_n)_{n=1}^\infty$$ is convergent and $$\lim\limits_{n \to \infty} s_n \leqslant \dfrac{1}{2}$$.

[//]: # _**Intuition**_

_**Proof**_

(WTS: $$(s_n)_{n=1}^\infty$$ is convergent $$\Longleftrightarrow (s_n)_{n=1}^\infty$$ is bounded
below and monotonic nonincreasing.)

We note that $$s_1 = \dfrac{1}{2}$$, $$s_2 = s_1 \cdot \dfrac{3}{4}$$ $$< s_1$$,
$$s_3 = s_2 \cdot \dfrac{5}{6}$$ $$< s_2$$, and in general,
$$s_k = s_{k - 1} \cdot \dfrac{2k - 1}{2k}$$ $$< s_{k - 1}$$
(since, $$\dfrac{2k - 1}{2k} < 1$$).

Hence, the sequence $$(s_n)_{n=1}^\infty$$ is nonincreasing; $$\dfrac{1}{2} = s_1$$
$$> s_2 > s_3$$ $$> \ldots > s_{k - 1}$$ $$> s_k > s_{k + 1}$$ $$> \ldots$$.

However, we also note that since $$s_1 = \dfrac{1}{2}$$, and that,
$$0 < \dfrac{2k - 1}{2k}$$ $$< 1$$, since, $$k > 0$$, the sequence is bounded
below by $$0$$.

Thus, $$(s_n)_{n=1}^\infty$$ is convergent.

Also, we note that $$\inf\{s_1, s_2, ..., s_k, s_{k + 1}, ...\} \leqslant \dfrac{1}{2}$$,
as $$s_1 = \dfrac{1}{2}$$. $$\blacksquare$$
