---
layout: subpage
title: Richard Goldberg Exercise 2.7 Q10(a)
description: Discusses the given question, the intuition behind the proof, and the proof itself
---

In this section, I will discuss the given question, the intuition behind the proof, and the
proof itself.

---

_**Question**_

Suppose $$s_1 > s_2$$ $$> 0$$, and let $$s_{n + 1} = \dfrac{1}{2} (s_n + s_{n - 1})$$
$$(n \geqslant 2)$$.

Prove that $$s_1, s_3, s_5, \ldots$$ is nonincreasing.

[//]: # _**Intuition**_

_**Proof**_

(Claim: $$(s_{2n - 1})_{n=1}^\infty$$ is nonincreasing, i.e,
$$s_{2n - 1} \geqslant s_{2n + 1}$$)

Base Case: $$k = 1$$

Then, $$s_3 = \dfrac{1}{2} (s_2 + s_1)$$
$$= \dfrac{1}{2} s_2 + \dfrac{1}{2} s_1 < \dfrac{1}{2}s_1 + \dfrac{1}{2} s_1$$
$$= s_1$$ (since $$s_1 > s_2$$).

Thus, $$s_3 \leqslant s_1$$, is true.

Inductive Step:

Inductively, assume that, $$s_{2k - 1} \geqslant s_{2k + 1}$$.

We note that, $$\dfrac{1}{2} (s_{2k - 1} + s_{2k}) \geqslant \dfrac{1}{2} (s_{2k + 1} + s_{2k})$$
$$\Longrightarrow s_{2k + 1} \geqslant s_{2k + 2}$$.

Thus, $$s_{2k + 3} = \dfrac{1}{2} (s_{2k + 2} + s_{2k + 1})$$
$$= \dfrac{1}{2} s_{2k + 2} + \dfrac{1}{2} s_{2k + 1} \leqslant \dfrac{1}{2} s_{2k + 1} + \dfrac{1}{2} s_{2k + 1}$$
$$= s_{2k + 1}$$ (since $$s_{2k + 1} \geqslant s_{2k + 2}$$).

Hence, $$s_{2k + 3} \leqslant s_{2k + 1}$$.

Thus, this shows that $$(s_{2n - 1})_{n=1}^\infty$$ is nonincreasing (decreasing).
$$\blacksquare$$
